enterM and leaveM proofs of correctness

Validator/Regex/EnterMem.lean
@@ -5,6 +5,27 @@ import Validator.Regex.Enter
 
 namespace Regex
 
-instance [Monad m] {σ: Type} [DecidableEq σ] [Hashable σ] [MonadState (MemTable enter (α := Regex σ)) m]:
+def enterM [DecidableEq σ] [Hashable σ] [Monad m] [MonadState (MemTable (@enter σ)) m]
+  (param: Regex σ): m { symbols // symbols = enter param } :=
+  callM enter param
+
+instance [DecidableEq σ] [Hashable σ] [Monad m] [MonadState (MemTable (@enter σ)) m]:
   Memoize m (α := Regex σ) (β := fun r => Vector σ (symbols r)) enter where
-  call r := callM enter r
+  call param := enterM param
+
+private theorem enterM_is_correct [DecidableEq σ] [Hashable σ] (param: Regex σ) (table: (MemTable (@enter σ))):
+  enter param = (StateM.run (s := table) (enterM param)).1 := by
+  have h := call_is_correct (@enter σ) table param
+  unfold call at h
+  unfold callM at h
+  unfold enterM
+  unfold callM
+  simp_state
+  cases Std.ExtDHashMap.get? table param with
+  | none =>
+    simp only
+    simp_state
+  | some res =>
+    obtain ⟨res, hres⟩ := res
+    simp_state
+    rw [hres]
