Validator/Regex/LeaveMem.lean
@@ -9,6 +9,27 @@ namespace Regex
 def leave2 {σ: Type}: (Σ (r: Regex σ), (Vector Bool (symbols r))) → Regex σ
   | ⟨r, bools⟩ => leave r bools
 
-instance [Monad m] {σ: Type} [DecidableEq σ] [Hashable σ] [MonadState (MemTable leave2 (α := (Σ (r: Regex σ), (Vector Bool (symbols r))))) m]:
+def leaveM {σ: Type} [DecidableEq σ] [Hashable σ] [Monad m] [MonadState (MemTable leave2 (α := (Σ (r: Regex σ), (Vector Bool (symbols r))))) m]
+  (param: Σ (r: Regex σ), (Vector Bool (symbols r))): m { res // res = leave2 param } :=
+  callM leave2 param
+
+instance {σ: Type} [DecidableEq σ] [Hashable σ] [Monad m] [MonadState (MemTable leave2 (α := (Σ (r: Regex σ), (Vector Bool (symbols r))))) m]:
   Memoize m (α := (Σ (r: Regex σ), (Vector Bool (symbols r)))) (β := fun _ => Regex σ) leave2 where
-  call r := callM leave2 r
+  call param := leaveM param
+
+private theorem leaveM_is_correct [DecidableEq σ] [Hashable σ] (param: Σ (r: Regex σ), (Vector Bool (symbols r))) (table: (MemTable (@leave2 σ))):
+  leave2 param = (StateM.run (s := table) (leaveM param)).1 := by
+  have h := call_is_correct (@leave2 σ) table param
+  unfold call at h
+  unfold callM at h
+  unfold leaveM
+  unfold callM
+  simp_state
+  cases Std.ExtDHashMap.get? table param with
+  | none =>
+    simp only
+    simp_state
+  | some res =>
+    obtain ⟨res, hres⟩ := res
+    simp_state
+    rw [hres]
