Validator/Std/State.lean
@@ -1,3 +1,5 @@
+import Lean.Elab.Tactic
+
 @[always_inline, inline, expose]
 def StateM.run {σ : Type u} {α : Type u} (x : StateM σ α) (s : σ) : α × σ :=
   x s
@@ -5,3 +7,23 @@ def StateM.run {σ : Type u} {α : Type u} (x : StateM σ α) (s : σ) : α × �
 @[always_inline, inline, expose]
 def StateM.run' {σ : Type u} {α : Type u} (x : StateM σ α) (s : σ) : α :=
   (·.1) <$> x s
+
+elab "simp_state" : tactic => do
+  Lean.Elab.Tactic.evalTactic (←
+  `(tactic| simp only [
+    getThe,
+    Bind.bind,
+    Functor.map,
+    MonadState.get,
+    MonadState.set,
+    MonadStateOf.get,
+    MonadStateOf.set,
+    Pure.pure,
+    StateT.bind,
+    StateT.get,
+    StateT.map,
+    StateT.pure,
+    StateT.run,
+    StateT.set,
+    StateM.run] at *
+  ))
